DeBruijnSSA/BinSyntax/Typing/Region/LSubst.lean
@@ -21,6 +21,11 @@ def Region.Subst.InS.get (r : Region.Subst.InS φ Γ L K) (i : Fin L.length)
   : Region.InS φ (⟨L.get i, ⊥⟩::Γ) K
   := ⟨r.1 i, r.2 i⟩
 
+@[simp]
+theorem Region.Subst.InS.coe_get (r : Region.Subst.InS φ Γ L K) (i : Fin L.length)
+  : (r.get i : Region φ) = r.1 i
+  := rfl
+
 instance Region.Subst.InS.instCoeOut {Γ : Ctx α ε} {L K : LCtx α}
   : CoeOut (Region.Subst.InS φ Γ L K) (Region.Subst φ)
   := ⟨λr => r.1⟩
@@ -58,16 +63,42 @@ theorem Region.Subst.InS.coe_lift (h : A ≤ A') (σ : Region.Subst.InS φ Γ L 
   : (σ.lift h : Region.Subst φ) = (σ : Region.Subst φ).lift
   := rfl
 
+@[simp]
+theorem Region.Subst.InS.get_lift_zero {σ : Region.Subst.InS φ Γ L K} {h : lo ≤ hi}
+  : (σ.lift h).get ⟨0, by simp⟩ = Region.InS.br 0 (Term.InS.var 0 Ctx.Var.shead) (by simp [h])
+  := rfl
+
+@[simp]
+theorem Region.Subst.InS.get_lift_succ
+  {σ : Region.Subst.InS φ Γ L K} {h : lo ≤ hi} {i : Fin L.length}
+  : (σ.lift h).get i.succ = (σ.get i).lwk0
+  := rfl
+
 def Region.Subst.WfD.slift {head} (hσ : σ.WfD Γ L K) : σ.lift.WfD Γ (head::L) (head::K)
   := hσ.lift (le_refl head)
 
 theorem Region.Subst.Wf.slift {head} (hσ : σ.Wf Γ L K) : σ.lift.Wf Γ (head::L) (head::K)
   := hσ.lift (le_refl head)
 
--- @[simp]
--- theorem Region.Subst.InS.coe_slift (σ : Region.Subst.InS φ Γ L K)
---   : (σ.slift : Region.Subst φ) = (σ : Region.Subst φ).slift A
---   := rfl
+def Region.Subst.InS.slift {head} (σ : Region.Subst.InS φ Γ L K)
+  : Region.Subst.InS φ Γ (head::L) (head::K)
+  := σ.lift (le_refl head)
+
+@[simp]
+theorem Region.Subst.InS.coe_slift (σ : Region.Subst.InS φ Γ L K)
+  : (σ.slift (head := head) : Region.Subst φ) = (σ : Region.Subst φ).lift
+  := rfl
+
+@[simp]
+theorem Region.Subst.InS.get_slift_zero {σ : Region.Subst.InS φ Γ L K}
+  : (σ.slift (head := head)).get (0 : Fin (L.length + 1))
+  = Region.InS.br 0 (Term.InS.var 0 Ctx.Var.shead) (by simp)
+  := rfl
+
+@[simp]
+theorem Region.Subst.InS.get_slift_succ {σ : Region.Subst.InS φ Γ L K} {i : Fin L.length}
+  : (σ.slift (head := head)).get i.succ = (σ.get i).lwk0
+  := rfl
 
 def Region.Subst.WfD.liftn_append (J : LCtx α) (hσ : σ.WfD Γ L K)
   : (σ.liftn J.length).WfD Γ (J ++ L) (J ++ K)
@@ -84,6 +115,29 @@ theorem Region.Subst.Wf.liftn_append (J : LCtx α) (hσ : σ.Wf Γ L K)
 def Region.Subst.InS.liftn_append (J : LCtx α) (σ : Region.Subst.InS φ Γ L K)
   : Region.Subst.InS φ Γ (J ++ L) (J ++ K)
   := ⟨σ.val.liftn J.length, σ.prop.liftn_append J⟩
+
+@[simp]
+theorem Region.Subst.InS.coe_liftn_append {Γ : Ctx α ε} {L K J : LCtx α}
+  {σ : Subst.InS φ Γ L K}
+  : (σ.liftn_append J : Region.Subst φ) = (σ : Region.Subst φ).liftn J.length
+  := rfl
+
+@[simp]
+theorem Region.Subst.InS.liftn_append_get_le {Γ : Ctx α ε} {L K J : LCtx α}
+  {σ : Subst.InS φ Γ L K} {i : Fin (J ++ L).length}
+  (h : i < J.length)
+  : (σ.liftn_append J).get i
+  = InS.br i (Term.InS.var 0 Ctx.Var.shead)
+    (LCtx.Trg.of_le_getElem
+      (by simp only [List.length_append]; omega)
+      (by simp [List.getElem_append_left, h]))
+  := by ext; simp [Region.Subst.liftn, h]
+
+@[simp]
+theorem Region.Subst.InS.liftn_append_singleton {Γ : Ctx α ε} {L K : LCtx α} {V : Ty α}
+  {σ : Subst.InS φ Γ L K}
+  : σ.liftn_append [V] = σ.slift
+  := by ext; simp [liftn_one]
 
 def Region.Subst.WfD.liftn_append' {J : LCtx α} (hn : n = J.length) (hσ : σ.WfD Γ L K)
   : (σ.liftn n).WfD Γ (J ++ L) (J ++ K)
@@ -110,6 +164,11 @@ theorem Region.Subst.Wf.vlift (hσ : σ.Wf Γ L K) : σ.vlift.Wf (head::Γ) L K
 def Region.Subst.InS.vlift (σ : Region.Subst.InS φ Γ L K) : InS φ (head::Γ) L K
   := ⟨Subst.vlift σ, σ.prop.vlift⟩
 
+@[simp]
+theorem Region.Subst.InS.coe_vlift (σ : Region.Subst.InS φ Γ L K)
+  : (σ.vlift (head := head) : Region.Subst φ) = Subst.vlift σ
+  := rfl
+
 def Region.Subst.WfD.vlift₂ (hσ : σ.WfD Γ L K) : σ.vlift.vlift.WfD (left::right::Γ) L K
   := hσ.vlift.vlift
 
@@ -121,6 +180,11 @@ theorem Region.Subst.Wf.vliftn₂ (hσ : σ.Wf Γ L K) : (σ.vliftn 2).Wf (left:
 
 def Region.Subst.InS.vliftn₂ (σ : Region.Subst.InS φ Γ L K) : InS φ (left::right::Γ) L K
   := ⟨Subst.vliftn 2 σ, σ.prop.vliftn₂⟩
+
+@[simp]
+theorem Region.Subst.InS.coe_vliftn₂ (σ : Region.Subst.InS φ Γ L K)
+  : (σ.vliftn₂ (left := left) (right := right) : Region.Subst φ) = Subst.vliftn 2 σ
+  := rfl
 
 theorem Region.Subst.InS.vliftn₂_eq_vlift_vlift (σ : Region.Subst.InS φ Γ L K)
   : σ.vliftn₂ (left := left) (right := right) = σ.vlift.vlift
@@ -191,6 +255,21 @@ theorem Region.Subst.Wf.comp {Γ : Ctx α ε} {σ : Region.Subst φ} {τ : Regio
   (hσ : σ.Wf Γ K J) (hτ : τ.Wf Γ L K) : (σ.comp τ).Wf Γ L J
   := λi => (hτ i).lsubst hσ.vlift
 
+def Region.Subst.InS.comp {Γ : Ctx α ε}
+  (σ : Region.Subst.InS φ Γ K J) (τ : Region.Subst.InS φ Γ L K) : Region.Subst.InS φ Γ L J
+  := ⟨σ.val.comp τ.val, σ.prop.comp τ.prop⟩
+
+@[simp]
+theorem Region.Subst.InS.coe_comp {Γ : Ctx α ε}
+  {σ : Region.Subst.InS φ Γ K J} {τ : Region.Subst.InS φ Γ L K}
+  : (σ.comp τ : Region.Subst φ) = (σ : Region.Subst φ).comp τ := rfl
+
+theorem Region.InS.lsubst_lsubst {Γ : Ctx α ε}
+  {σ : Region.Subst.InS φ Γ K J} {τ : Region.Subst.InS φ Γ L K}
+  {r : Region.InS φ Γ L}
+  : (r.lsubst τ).lsubst σ = r.lsubst (σ.comp τ)
+  := by ext; simp [Region.lsubst_lsubst]
+
 def Region.Subst.InS.vsubst {Γ Δ : Ctx α ε}
   (ρ : Term.Subst.InS φ Γ Δ) (σ : Region.Subst.InS φ Δ L K)
   : Region.Subst.InS φ Γ L K
@@ -221,6 +300,86 @@ theorem LCtx.InS.coe_toSubst {Γ : Ctx α ε} {L K : LCtx α} {ρ : L.InS K}
 def Region.InS.lsubst_toSubst {Γ : Ctx α ε} {L K : LCtx α} {ρ : L.InS K} {r : Region.InS φ Γ L}
   : r.lsubst (ρ.toSubst) = r.lwk ρ
   := by ext; simp [Region.lsubst_fromLwk]
+
+@[simp]
+theorem Region.InS.get_toSubst {Γ : Ctx α ε} {L K : LCtx α} {ρ : L.InS K} {ℓ : Fin L.length}
+  : ((ρ.toSubst (φ := φ) (Γ := Γ)).get ℓ)
+  = InS.br (ρ.val ℓ) (Term.InS.var 0 Ctx.Var.shead) (ρ.prop ℓ ℓ.prop)
+  := rfl
+
+@[simp]
+theorem Region.InS.lsubst_br {Γ : Ctx α ε} {L K : LCtx α} {σ : Subst.InS φ Γ L K}
+  {ℓ : ℕ} {a : Term.InS φ Γ ⟨A, ⊥⟩} {hℓ : L.Trg ℓ A}
+  : (br ℓ a hℓ).lsubst σ = ((σ.get ⟨ℓ, hℓ.length⟩).vwk_id (by simp [hℓ.getElem])).vsubst a.subst0
+  := rfl
+
+@[simp]
+theorem Region.InS.lsubst_case {Γ : Ctx α ε} {L K : LCtx α} {σ : Subst.InS φ Γ L K}
+  {e : Term.InS φ Γ (A.coprod B, ⊥)}
+  {s : Region.InS φ ((A, ⊥)::Γ) L} {t : Region.InS φ ((B, ⊥)::Γ) L}
+  : (case e s t).lsubst σ = case e (s.lsubst σ.vlift) (t.lsubst σ.vlift)
+  := rfl
+
+@[simp]
+theorem Region.InS.lsubst_let1 {Γ : Ctx α ε} {L K : LCtx α} {σ : Subst.InS φ Γ L K}
+  {a : Term.InS φ Γ ⟨A, e⟩} {t : Region.InS φ ((A, ⊥)::Γ) L}
+  : (let1 a t).lsubst σ = let1 a (t.lsubst σ.vlift)
+  := rfl
+
+@[simp]
+theorem Region.InS.lsubst_let2 {Γ : Ctx α ε} {L K : LCtx α} {σ : Subst.InS φ Γ L K}
+  {a : Term.InS φ Γ ⟨A.prod B, e⟩} {t : Region.InS φ ((B, ⊥)::(A, ⊥)::Γ) L}
+  : (let2 a t).lsubst σ = let2 a (t.lsubst σ.vliftn₂)
+  := rfl
+
+@[simp]
+theorem Region.InS.lsubst_cfg {Γ : Ctx α ε} {L K : LCtx α} {σ : Subst.InS φ Γ L K}
+  {R : LCtx α} {β : Region.InS φ Γ (R ++ L)}
+  {G : ∀i : Fin R.length, Region.InS φ ((R.get i, ⊥)::Γ) (R ++ L)}
+  : (cfg R β G).lsubst σ
+  = cfg R (β.lsubst (σ.liftn_append R)) (λi => (G i).lsubst (σ.liftn_append R).vlift)
+  := rfl
+
+theorem Region.InS.lsubst_lift_lwk0 {Γ : Ctx α ε} {L K : LCtx α}
+  {σ : Subst.InS φ Γ L K} {h : lo ≤ hi} {r : Region.InS φ Γ L}
+  : r.lwk0.lsubst (σ.lift h) = (r.lsubst σ).lwk0 := by
+  ext
+  simp only [coe_lsubst, Subst.InS.coe_lift, coe_lwk0, Region.lwk0, ←lsubst_fromLwk,
+    Region.lsubst_lsubst]
+  congr
+  funext k
+  simp only [Subst.comp, Region.lsubst, Subst.vlift, Nat.succ_eq_add_one,
+    Function.comp_apply, Subst.lift, Region.Subst.vwk1_comp_fromLwk]
+  simp only [<-Region.vsubst_fromWk, Region.vwk1, Region.vsubst_vsubst]
+  rw [Region.vsubst_id', Region.lsubst_fromLwk]
+  funext k
+  cases k <;> rfl
+
+theorem Region.InS.lsubst_slift_lwk0 {Γ : Ctx α ε} {L K : LCtx α}
+  {σ : Subst.InS φ Γ L K} {r : Region.InS φ Γ L}
+  : r.lwk0.lsubst (σ.slift (head := head)) = (r.lsubst σ).lwk0 := Region.InS.lsubst_lift_lwk0
+
+theorem Region.Subst.InS.vlift_lift {Γ : Ctx α ε} {L K : LCtx α}
+  {σ : Subst.InS φ Γ L K} {h : lo ≤ hi}
+  : (σ.lift h).vlift (head := head) = σ.vlift.lift h := by ext; simp [Region.Subst.vlift_lift_comm]
+
+theorem Region.Subst.InS.vlift_slift {Γ : Ctx α ε} {L K : LCtx α}
+  {σ : Subst.InS φ Γ L K}
+  : (σ.slift (head := head')).vlift (head := head) = σ.vlift.slift := vlift_lift
+
+theorem Region.InS.vwk1_lsubst_vlift {Γ : Ctx α ε} {L K : LCtx α}
+  {σ : Subst.InS φ Γ L K} {r : Region.InS φ (head::Γ) L}
+  : (r.lsubst σ.vlift).vwk1 (inserted := inserted) = r.vwk1.lsubst σ.vlift.vlift := by
+  ext
+  simp only [Set.mem_setOf_eq, vwk1, coe_vwk, Ctx.InS.coe_wk1, coe_lsubst, Subst.InS.coe_vlift,
+    Subst.vlift, vwk_lsubst]
+  congr
+  simp only [<-Function.comp.assoc, Region.vwk1, <-Region.vwk_comp]
+  apply congrFun
+  apply congrArg
+  apply congrArg
+  funext k
+  cases k <;> rfl
 
 end RegionSubst
 
